---
published: true
mathjax: true
mathjax_autoNumber: true
---

## A New Post

When $$a \ne 0$$, there are two solutions to $$ax^2 + bx + c = 0$$ and they are

$$x_1 = {-b + \sqrt{b^2-4ac} \over 2a}$$


$$x_2 = {-b - \sqrt{b^2-4ac} \over 2a}$$


![image]({{site.baseurl}}/assets/images/1.jpg){:width="128px" height="128px"}
![image]({{site.baseurl}}/assets/images/1.jpg)
![image]({{site.baseurl}}/assets/images/1.jpg){:width="64px" height="64px"}




Enter text in [Markdown](http://daringfireball.net/projects/markdown/). Use the toolbar above, or click the **?** button for formatting help.
